LambdaGraph/Lemmas.lean
@@ -12,13 +12,34 @@ theorem value_types_bool {L : Type} {p : Program L} {Γ : List L} {v : Expr L}
   · cases ht
   · exists b
 
+theorem types_in_superset {L : Type} {p : Program L} {Γ Γ' : List L}
+  {e : Expr L} {t : Ty} (h : p / Γ ⊢ e : t) (hs : Γ ⊆ Γ') : p / Γ' ⊢ e : t := by
+  induction h generalizing Γ' with try solve | constructor <;> apply_rules
+  | fnNew Γ l h ih =>
+    apply Types.fnNew
+    apply ih
+    simp [hs]
+
+theorem types_subst {L : Type} {p : Program L} {Γ : List L} {e : Expr L}
+  {t : Ty} {σ : Env L} (hΓ : ∀ l ∈ Γ, p / Γ ⊢ p.fn l : .bot)
+  (h : p / Γ ⊢ e : t) (hσ : ∀ l ∈ Γ, p / [] ⊢ σ l : p.ty l) :
+    p / [] ⊢ e.subst σ : t := by
+  induction h with try solve | (try constructor) <;> apply_rules
+  | fnRec Γ l hl =>
+    constructor
+    · apply types_in_superset (hΓ l hl)
+      change Γ ⊆ l :: Γ
+      simp
+    · exact hΓ
+    · exact hσ
+
 theorem progress {L : Type} [DecidableEq L] {p : Program L} {e : Expr L}
   {t : Ty} (h : p / [] ⊢ e : t) : e.Value ∨ ∃ e', p / e ⇒ e' := by
   generalize hΓ : [] = Γ at h
   induction h with subst hΓ
   | var Γ l hl => simp at hl
   | fnRec Γ l hl => simp at hl
-  | fnNew Γ l hl h ih => right; repeat constructor
+  | fnNew Γ l h ih => right; repeat constructor
   | app Γ f e t hf he ihf ihe =>
     right
     rcases ihf rfl with hvf | ⟨f', hsf⟩
@@ -35,3 +56,24 @@ theorem progress {L : Type} [DecidableEq L] {p : Program L} {e : Expr L}
     · obtain ⟨b, rfl⟩ := value_types_bool hc hvc
       cases b <;> repeat constructor
     · exact ⟨_, Step.condC _ _ _ _ hsc⟩
+
+theorem preservation {L : Type} [DecidableEq L] {p : Program L} {e e' : Expr L}
+  {t : Ty} (h : p / [] ⊢ e : t) (hs : p / e ⇒ e') : p / [] ⊢ e' : t := by
+  induction hs generalizing t with
+    try solve | cases h <;> apply_rules [Types.app, Types.cond]
+  | fn l =>
+    cases h <;> constructor <;> intros <;> apply_rules [List.not_mem_nil]
+  | app l σ e hve =>
+    cases h with
+    | app _ _ _ t h he =>
+      cases h with
+      | clos _ Γ _ _ h hΓ hσ =>
+        apply types_subst (Γ := l :: Γ)
+        · rintro l' (_ | ⟨_, hl'⟩)
+          · exact h
+          · exact types_in_superset (hΓ l' hl') (by simp)
+        · exact h
+        · rintro l' (_ | ⟨_, hl'⟩)
+          · simp [he, Env.update]
+          · simp only [Env.update]
+            split <;> subst_eqs <;> apply_rules
